vale/code/arch/x64/X64.Leakage_Ins_Xmm.fst
@@ -13,8 +13,9 @@ open X64.Bytes_Semantics
 
 let xmm_taint (ts:taintState) (x:xmm) = ts.xmmTaint x
 
-let set_xmm_taint (ts:taintState) (xmm:xmm) (taint:taint) : taintState =
-  TaintState ts.regTaint ts.flagsTaint ts.cfFlagsTaint (fun x -> if x = xmm then taint else ts.xmmTaint x)
+let set_xmm_taint (ts:taintState) (xmm_v:xmm) (taint:taint) : taintState =
+  TaintState ts.regTaint ts.flagsTaint ts.cfFlagsTaint 
+    (FunctionalExtensionality.on xmm (fun x -> if x = xmm_v then taint else ts.xmmTaint x))
 
 #reset-options "--initial_ifuel 2 --max_ifuel 2 --initial_fuel 4 --max_fuel 4 --z3rlimit 80"
 
